src/tidy/rewrite_search/interactive.lean
@@ -7,24 +7,24 @@ import .discovery
 
 namespace tactic.interactive
 
-open lean.parser interactive
+open lean.parser interactive interactive.types
 open tidy.rewrite_search
 
 variables {α β γ δ : Type}
 
-meta def rewrite_search (try_harder : parse $ optional (tk "!")) (cfg : rewrite_search_config α β γ δ . pick_default_config) : tactic string :=
+meta def rewrite_search (try_harder : parse $ optional (tk "!")) (cfg : iconfig.rewrite_search.interactive.itactic) : tactic string :=
   tactic.rewrite_search cfg try_harder.is_some
 
-meta def rewrite_search_with (try_harder : parse $ optional (tk "!")) (rs : parse rw_rules) (cfg : rewrite_search_config α β γ δ . pick_default_config) : tactic string :=
+meta def rewrite_search_with (try_harder : parse $ optional (tk "!")) (rs : parse rw_rules) (cfg : iconfig rewrite_search) : tactic string :=
   tactic.rewrite_search_with rs.rules cfg try_harder.is_some
 
-meta def rewrite_search_using (try_harder : parse $ optional (tk "!")) (as : list name) (cfg : rewrite_search_config α β γ δ . pick_default_config) : tactic string :=
+meta def rewrite_search_using (try_harder : parse $ optional (tk "!")) (as : list name) (cfg : iconfig rewrite_search) : tactic string :=
   tactic.rewrite_search_using as cfg try_harder.is_some
 
-meta def simp_search (cfg : rewrite_search_config α β γ δ . pick_default_config) : tactic unit :=
+meta def simp_search (cfg : iconfig rewrite_search) : tactic unit :=
   tactic.simp_search cfg
 
-meta def simp_search_with (rs : parse rw_rules) (cfg : rewrite_search_config α β γ δ . pick_default_config) : tactic unit :=
+meta def simp_search_with (rs : parse rw_rules) (cfg : iconfig rewrite_search := tactic.skip) : tactic unit :=
   tactic.simp_search_with rs.rules cfg
 
 end tactic.interactive
