src/tidy/rewrite_search/metric/edit_distance/core.lean
@@ -1,4 +1,5 @@
 import tidy.rewrite_search.core
+import tidy.rewrite_search.module
 
 import data.rat
 
@@ -67,19 +68,25 @@ namespace tidy.rewrite_search.metric.edit_distance
 
 open tidy.rewrite_search.edit_distance
 
+@[derive has_reflect]
 structure ed_config :=
 (refresh_freq     : ℕ := 10)
 (explain_thoughts : bool := ff)
 (trace_weights    : bool := ff)
 
 structure ed_state :=
-  (weights : table dnum)
-def ed_state.init : ed_state := ⟨table.create⟩
+(cfg     : ed_config)
+(weights : table dnum)
+def ed_state.init (cfg : ed_config := {}) : ed_state := ⟨cfg, table.create⟩
 
 -- In future we might allow init_fn to return some internal weight state. At
 -- the moment, it is just used to ensure that an external depedency (e.g.
 -- external program or custom lean fork) is present.
-meta def calc_weights_fn (α δ : Type) := ed_config → search_state α ed_state ed_partial δ → tactic (table dnum)
+meta def calc_weights_fn (α δ : Type) := search_state α ed_state ed_partial δ → tactic (table dnum)
+
+meta structure calc_weights_block :=
+(α δ : Type)
+(fn : calc_weights_fn α δ)
 
 meta structure ed_weight (α δ : Type) :=
 (init : init_fn unit)
@@ -87,11 +94,15 @@ meta structure ed_weight (α δ : Type) :=
 
 meta def ed_weight_constructor := Π α δ, ed_weight α δ
 
-variables {α δ : Type} (g : search_state α ed_state ed_partial δ) (conf : ed_config)
+variables {α δ : Type} (g : search_state α ed_state ed_partial δ)
 
-meta def ed_init (weight_init : init_fn unit) : tactic (init_result ed_state) := do
+meta def ed_init (cfg : ed_config) (weight_init : init_fn unit) : tactic (init_result ed_state) := do
   init_result.chain "weight" weight_init $ λ _,
-    init_result.pure ed_state.init
+    init_result.pure $ ed_state.init cfg
+
+meta def ed_decode (icfg : iconfig.result) (w : init_fn unit) : tactic (init_result ed_state) := do
+  cfg ← icfg.struct `tidy.rewrite_search.metric.edit_distance.ed_config ed_config,
+  ed_init cfg w
 
 meta def ed_init_bound (l r : vertex) : bound_progress ed_partial :=
   at_least 0 (empty_partial_edit_distance_data g.metric_state.weights l.tokens r.tokens)
@@ -99,19 +110,19 @@ meta def ed_init_bound (l r : vertex) : bound_progress ed_partial :=
 meta def ed_reweight (fn : search_state α ed_state ed_partial δ → tactic (table dnum)) (g : search_state α ed_state ed_partial δ) : tactic (search_state α ed_state ed_partial δ) := do
   g ← g.reset_all_estimates ed_init_bound,
   weights ← fn g,
-  if conf.trace_weights then
+  if g.metric_state.cfg.trace_weights then
     let weight_pairs := (g.tokens.to_list.zip weights.to_list).map (
       λ p : token × dnum, to_string format!"{p.1.str}={p.2}"
     ) in
     tactic.trace format!"reweighted: {weight_pairs}"
   else
     tactic.skip,
-  return $ g.mutate_metric ⟨weights⟩
+  return $ g.mutate_metric {g.metric_state with weights := weights}
 
-meta def ed_update (fn : search_state α ed_state ed_partial δ → tactic (table dnum)) (g : search_state α ed_state ed_partial δ) (itr : ℕ) : tactic (search_state α ed_state ed_partial δ) :=
-  if conf.refresh_freq > 0 ∧ (itr % (conf.refresh_freq + 1) = 0) then do
-    if conf.explain_thoughts then tactic.trace "pause! refreshing weights..." else tactic.skip,
-    ed_reweight conf fn g
+meta def ed_update (fn : calc_weights_fn α δ) (g : search_state α ed_state ed_partial δ) (itr : ℕ) : tactic (search_state α ed_state ed_partial δ) :=
+  if g.metric_state.cfg.refresh_freq > 0 ∧ (itr % (g.metric_state.cfg.refresh_freq + 1) = 0) then do
+    if g.metric_state.cfg.explain_thoughts then tactic.trace "pause! refreshing weights..." else tactic.skip,
+    ed_reweight fn g
   else
     return g
 
@@ -119,16 +130,3 @@ meta def ed_improve_estimate_over (g : search_state α ed_state ed_partial δ) (
   improve_bound_over m bnd
 
 end tidy.rewrite_search.metric.edit_distance
-
-namespace tidy.rewrite_search.metric
-open tidy.rewrite_search.edit_distance
-open tidy.rewrite_search.metric.edit_distance
-
-meta def weight.none : ed_weight_constructor :=
-  λ α δ, ⟨init_result.pure (), λ conf g, return table.create⟩
-
-meta def edit_distance (conf : ed_config := {}) (w_cons : ed_weight_constructor := weight.none) : metric_constructor ed_state ed_partial :=
-  λ α δ, let w := w_cons α δ in
-  ⟨ ed_init w.init, ed_update conf $ w.calc_weights conf, ed_init_bound, ed_improve_estimate_over ⟩
-
-end tidy.rewrite_search.metric
