src/tidy/rewrite_search/tracer/unit.lean
@@ -1,4 +1,6 @@
+import tactic.iconfig
 import tidy.rewrite_search.core
+import tidy.rewrite_search.module
 
 open tidy.rewrite_search
 
@@ -20,9 +22,19 @@ namespace tidy.rewrite_search.tracer
 
 open tidy.rewrite_search.tracer.unit
 
-meta def unit_tracer : tracer_constructor unit := λ α β γ,
+meta def no_cfg (_ : name) (_ : interactive.parse interactive.types.texpr) : cfgtactic unit := tactic.skip
+
+iconfig_add rewrite_search [ no : custom no_cfg ]
+
+meta def unit_cnst := λ α β γ,
   tracer.mk α β γ unit_tracer_init unit_tracer_publish_vertex unit_tracer_publish_edge unit_tracer_publish_visited unit_tracer_publish_finished unit_tracer_dump unit_tracer_pause
 
-meta def no {δ : Type} (_ : tracer_constructor δ) : tracer_constructor unit := unit_tracer
+meta def unit : tactic expr :=
+  generic `tidy.rewrite_search.tracer.unit_cnst
+
+meta def unit_cfg (_ : name) : cfgtactic _root_.unit :=
+  iconfig.publish `tracer $ cfgopt.value.pexpr $ expr.const `unit []
+
+iconfig_add rewrite_search [ tracer.unit : custom unit_cfg ]
 
 end tidy.rewrite_search.tracer
