src/tidy/rewrite_search/discovery/types.lean
@@ -7,12 +7,14 @@ universe u
 
 namespace tidy.rewrite_search.discovery
 
+open tidy.rewrite_search
+
 meta def discovery_trace {α : Type u} [has_to_tactic_format α] (a : α) (nl : bool := tt) : tactic unit := do
   str ← tactic.pp a,
   let nlc := if nl then "\n" else "",
   cur ← tactic.decl_name,
   tactic.trace format!"(discovery@{cur}): {str}{nlc}"
 
-meta def collector := config → progress → list expr → tactic (progress × list (expr × bool))
+meta def collector := config → list (expr × bool) → progress → list expr → tactic (progress × list (expr × bool))
 
 end tidy.rewrite_search.discovery
