src/tidy/rewrite_search/metric/edit_distance/default.lean
@@ -1,0 +1,44 @@
+import tidy.rewrite_search.core
+import tidy.rewrite_search.module
+
+import .core
+import .cm
+import .svm
+
+open tidy.rewrite_search
+open tidy.rewrite_search.bound_progress
+
+namespace tidy.rewrite_search.metric
+open tidy.rewrite_search.edit_distance
+open tidy.rewrite_search.metric.edit_distance
+
+meta def weight.none : ed_weight_constructor :=
+  λ α δ, ⟨init_result.pure (), λ g, return table.create⟩
+
+-- TODO I'm ugly
+meta def edit_distance_cnst (conf : iconfig.result) (n : option name) := λ α δ,
+  let w := match n with
+  | some `cm := weight.cm
+  | some `svm := weight.svm
+  | _ := weight.none
+  end in
+  @metric.mk α ed_state ed_partial δ (ed_decode conf (w α δ).init) (ed_update (w α δ).calc_weights) ed_init_bound ed_improve_estimate_over
+
+meta def edit_distance (conf : iconfig.result := iconfig.empty_result) (weight : option name := none) : tactic expr :=
+  generic_args ``tidy.rewrite_search.metric.edit_distance_cnst [`(conf), `(weight)]
+
+section
+
+iconfig_mk edit_distance
+iconfig_add_struct edit_distance tidy.rewrite_search.metric.edit_distance.ed_config
+
+meta def edit_distance_cfg (_ : name) (cfg : iconfig edit_distance) (w : interactive.parse (optional lean.parser.ident)) : cfgtactic unit := do
+  cfg ← iconfig.read cfg,
+  e ← tactic.to_expr $ ``(edit_distance) (pexpr.of_expr `(cfg)) (pexpr.of_expr `(w)),
+  iconfig.publish `metric $ cfgopt.value.pexpr $ pexpr.of_expr e
+
+iconfig_add rewrite_search [ metric.edit_distance : custom edit_distance_cfg ]
+
+end
+
+end tidy.rewrite_search.metric
