src/tidy/rewrite_search/strategy/bfs.lean
@@ -1,4 +1,6 @@
+import tactic.iconfig
 import tidy.rewrite_search.core
+import tidy.rewrite_search.module
 
 open tidy.rewrite_search
 
@@ -8,19 +10,21 @@ structure bfs_config :=
 (max_depth : ℕ := 50)
 
 structure bfs_state :=
+(conf       : bfs_config)
 (curr_depth : ℕ)
 (queue      : list (option table_ref))
 
-variables {β γ δ : Type} (conf : bfs_config) (g : search_state bfs_state β γ δ)
+variables {β γ δ : Type} (g : search_state bfs_state β γ δ)
 
-meta def bfs_init : tactic (init_result bfs_state) := init_result.pure ⟨1, []⟩
+meta def bfs_init : tactic (init_result bfs_state) := init_result.pure ⟨{}, 1, []⟩
 
-meta def bfs_startup (m : metric bfs_state β γ δ) (l r : vertex) : tactic (search_state bfs_state β γ δ) :=
-  return $ g.mutate_strat ⟨ 1, [l.id, r.id, none] ⟩
+meta def bfs_startup (cfg : iconfig.result) (g : search_state bfs_state β γ δ) (m : metric bfs_state β γ δ) (l r : vertex) : tactic (search_state bfs_state β γ δ) := do
+  cfg ← cfg.struct `tidy.rewrite_search.strategy.bfs.bfs_config bfs_config,
+  return $ g.mutate_strat ⟨cfg, 1, [l.id, r.id, none]⟩
 
 meta def bfs_step (g : search_state bfs_state β γ δ) (_ : metric bfs_state β γ δ) (_: ℕ) : tactic (search_state bfs_state β γ δ × status) := do
   let state := g.strat_state,
-  if state.curr_depth > conf.max_depth then
+  if state.curr_depth > g.strat_state.conf.max_depth then
     return (g, status.abort "max bfs depth reached!")
   else match state.queue with
   | [] := return (g, status.abort "all vertices exhausted!")
@@ -40,7 +44,23 @@ namespace tidy.rewrite_search.strategy
 
 open tidy.rewrite_search.strategy.bfs
 
-meta def bfs (conf : bfs_config := {}) : strategy_constructor bfs_state :=
-λ β γ δ, strategy.mk bfs_init (@bfs_startup β γ δ) (@bfs_step β γ δ conf)
+meta def bfs_const (conf : iconfig.result) := λ β γ δ, strategy.mk bfs_init (@bfs_startup β γ δ conf) (@bfs_step β γ δ)
+
+meta def bfs (conf : iconfig.result := iconfig.empty_result) : tactic expr :=
+  generic_arg `tidy.rewrite_search.strategy.bfs_const `(conf)
+
+section
+
+iconfig_mk bfs
+iconfig_add_struct bfs tidy.rewrite_search.strategy.bfs.bfs_config
+
+meta def bfs_cfg (_ : name) (cfg : iconfig bfs) : cfgtactic unit := do
+  cfg ← iconfig.read cfg,
+  e ← tactic.to_expr $ ``(bfs) $ pexpr.of_expr `(cfg),
+  iconfig.publish `strategy $ cfgopt.value.pexpr $ pexpr.of_expr e
+
+iconfig_add rewrite_search [ strategy.bfs : custom bfs_cfg ]
+
+end
 
 end tidy.rewrite_search.strategy
