test/rewrite_search.lean
@@ -1,9 +1,5 @@
 import tidy.rewrite_search
 
-open tidy.rewrite_search.metric
-open tidy.rewrite_search.strategy
-open tidy.rewrite_search.tracer
-
 namespace tidy.rewrite_search.testing
 
 axiom foo' : [6] = [7]
@@ -20,7 +16,7 @@ end
 
 example : [[7],[6]] = [[5],[5]] :=
 begin
- success_if_fail { rewrite_search_with [] },
+ success_if_fail { rewrite_search_with [] {} },
 -- rw [←foo', bar']
  rewrite_search_with [←foo', bar'] {explain := tt},
 end
@@ -57,8 +53,10 @@ end
 
 private example (a : unit) : [[0],[0]] = [[4],[4]] :=
 begin
-  rewrite_search_with [foo, bar1, ← bar2, bar2, ← bar3],
+  rewrite_search_with [foo, bar1, ← bar2, bar2, ← bar3] {strategy.pexplore {}, metric.edit_distance {}, no visualiser},
 end
+
+meta instance has_coe : has_coe iconfig.rewrite_search.interactive.itactic (opt_param iconfig.rewrite_search.interactive.itactic tactic.skip) := ⟨λ s, s⟩
 
 private example : [[0],[0]] = [[4],[4]] :=
 begin
@@ -76,8 +74,10 @@ begin
 -- conv { to_lhs, congr, rw [foo, bar1], skip, rw [foo, bar1] },
 -- conv { to_rhs, congr, rw [←bar3, bar2], skip, rw [←bar3, bar2] },
 
-  rewrite_search,
+  rewrite_search {metric.edit_distance {}, strategy.pexplore {}, no visualiser,}
 end
+
+#check tidy.rewrite_search.strategy.bfs
 
 @[search] private axiom qux' : [[1], [2]] = [[6], [7]]
 @[search] private axiom qux'' : [6] = [7]
@@ -86,7 +86,7 @@ begin
 -- nth_rewrite_lhs 0 bar1,
 -- nth_rewrite_lhs 0 qux',
 -- nth_rewrite_rhs 1 ←qux'',
-  rewrite_search {view := no visualiser}, -- FIXME this is broken until we can do single replacements.
+  rewrite_search {tracer.unit}, -- FIXME this is broken until we can do single replacements.
 end
 
 private example : [[0],[0]] = [[4],[4]] :=
@@ -164,7 +164,7 @@ run_cmd do all_rewrites_lazy (`(g_0_0), tt) `(g 0 0 0)
 
 lemma test : f 0 0 0 = g 0 0 0 :=
 -- by erw [f_2_2, f_1_1, g_0_2, g_2_1, ←f_g]
-by rewrite_search {trace := ff, explain := tt, trace_summary := tt, exhaustive := tt, view := no visualiser, strategy := pexplore {pop_size := 1}, metric := edit_distance {refresh_freq := 5} weight.cm}
+by rewrite_search {trace := ff, explain := tt, trace_summary := tt, exhaustive := tt, tracer.unit, strategy.pexplore {pop_size := 1}, metric.edit_distance {refresh_freq := 5} cm}
 -- begin
 -- perform_nth_rewrite [f_2_2] 0,
 -- perform_nth_rewrite [f_1_1] 0,
@@ -176,22 +176,22 @@ by rewrite_search {trace := ff, explain := tt, trace_summary := tt, exhaustive :
 
 lemma test_bfs : f 0 0 0 = g 0 0 0 :=
 -- by erw [f_2_2, f_1_1, g_0_2, g_2_1, ←f_g]
-by rewrite_search {trace := ff, explain := tt, trace_summary := tt, exhaustive := tt, view := no visualiser, strategy := pexplore {pop_size:=5}, metric := edit_distance {} weight.svm }
+by rewrite_search {trace := ff, explain := tt, trace_summary := tt, exhaustive := tt, no visualiser, strategy.pexplore {pop_size:=5}, metric.edit_distance {} svm }
 
 -- Compare: in these next two we just change pop_size 1 -> 5, and we find a much much
 -- better proof, but we see a little more stuff.
 
 lemma test_svm : f 0 0 0 = g 0 0 0 :=
 -- by erw [f_2_2, f_1_1, g_0_2, g_2_1, ←f_g]
-by rewrite_search {trace := ff, explain := tt, trace_summary := tt, exhaustive := tt, view := no visualiser, strategy := pexplore {pop_size := 1}, metric := edit_distance {refresh_freq := 1} weight.svm}
+by rewrite_search {trace := ff, explain := tt, trace_summary := tt, exhaustive := tt, no visualiser, strategy.pexplore {pop_size := 1}, metric.edit_distance {refresh_freq := 1} svm}
 
 lemma test_svm2 : f 0 0 0 = g 0 0 0 :=
 -- by erw [f_2_2, f_1_1, g_0_2, g_2_1, ←f_g]
-by rewrite_search {trace := ff, explain := tt, trace_summary := tt, exhaustive := tt, view := no visualiser, strategy := pexplore {pop_size := 5}, metric := edit_distance {refresh_freq := 1} weight.svm}
+by rewrite_search {trace := ff, explain := tt, trace_summary := tt, exhaustive := tt, no visualiser, strategy.pexplore {pop_size := 5}, metric.edit_distance {refresh_freq := 1} svm}
 
 lemma test_cm2 : f 0 0 0 = g 0 0 0 :=
 -- by erw [f_2_2, f_1_1, g_0_2, g_2_1, ←f_g]
-by rewrite_search {trace := ff, explain := tt, trace_summary := tt, exhaustive := tt, view := no visualiser, strategy := pexplore {pop_size := 5}, metric := edit_distance {refresh_freq := 1} weight.cm}
+by rewrite_search {trace := ff, explain := tt, trace_summary := tt, exhaustive := tt, no visualiser, strategy.pexplore {pop_size := 5}, metric.edit_distance {refresh_freq := 1} cm}
 
 constant h : ℕ → ℕ
 @[search,simp] axiom a1 : h 0 = h 1
@@ -201,15 +201,15 @@ constant h : ℕ → ℕ
 
 lemma test2 : h 0 = h 4 :=
 -- by erw [a1, a2, ←a4, ←a3]
-by rewrite_search
+by rewrite_search {}
 
 constants a b c d e : ℚ
 
 lemma test3 : (a * (b + c)) * d = a * (b * d) + a * (c * d) :=
-by rewrite_search_with [add_comm, add_assoc, mul_assoc, mul_comm, left_distrib, right_distrib] {explain := tt, trace_summary := tt, view := no visualiser, metric := edit_distance}
+by rewrite_search_with [add_comm, add_assoc, mul_assoc, mul_comm, left_distrib, right_distrib] {explain := tt, trace_summary := tt, no visualiser, metric.edit_distance {}}
 
 -- lemma test4 : (a * (b + c + 1)) * d = a * (b * d) + a * (1 * d) + a * (c * d) :=
--- by rewrite_search_with [add_comm, add_assoc, mul_one, mul_assoc, mul_comm, left_distrib, right_distrib] {explain := tt, trace_summary := tt, view := visualiser, metric := edit_distance {refresh_freq := 10} weight.cm, strategy := pexplore {pop_size := 3}, max_iterations := 1000}
+-- by rewrite_search_with [add_comm, add_assoc, mul_one, mul_assoc, mul_comm, left_distrib, right_distrib] {explain := tt, trace_summary := tt, view := visualiser, metric.edit_distance {refresh_freq := 10} cm, strategy.pexplore {pop_size := 3}, max_iterations := 1000}
 
 namespace tidy.rewrite_search.tesseract
 
@@ -270,7 +270,7 @@ namespace v1
 -- rewrite_search_with (saw/visited/used) 114/112/13 expressions during proof of tidy.rewrite_search.examples.tidy.rewrite_search.tesseract.v1.test
 lemma test : f_1 0 0 0 = f_5 0 0 0 :=
 -- by erw [f_2_2, f_1_1, g_0_2, g_2_1, ←f_g]
-by rewrite_search {trace := ff, explain := tt, trace_summary := tt, exhaustive := ff, view := no visualiser, strategy := pexplore {pop_size := 1, pop_alternate := ff}, metric := edit_distance, max_iterations := 1000}
+by rewrite_search {trace := ff, explain := tt, trace_summary := tt, exhaustive := ff, no visualiser, strategy.pexplore {pop_size := 1, pop_alternate := ff}, metric.edit_distance {}, max_iterations := 1000}
 end v1
 
 namespace v2
@@ -282,7 +282,7 @@ namespace v2
 
 -- lemma test : f_1 0 0 0 = f_5 0 0 0 :=
 -- -- by erw [f_2_2, f_1_1, g_0_2, g_2_1, ←f_g]
--- by rewrite_search {trace := ff, explain := tt, trace_summary := tt, exhaustive := ff, view := no visualiser, strategy := pexplore { pop_size := 100 }, metric := edit_distance {refresh_freq := 5} weight.cm}
+-- by rewrite_search {trace := ff, explain := tt, trace_summary := tt, exhaustive := ff, no visualiser, strategy.pexplore { pop_size := 100 }, metric.edit_distance {refresh_freq := 5} cm}
 end v2
 
 end tidy.rewrite_search.tesseract
