test/rewrite_search_vs_ring.lean
@@ -1,10 +1,6 @@
 import tactic.ring
 import tidy.rewrite_search
 
-open tidy.rewrite_search.metric
-open tidy.rewrite_search.strategy
-open tidy.rewrite_search.tracer
-
 namespace tidy.rewrite_search.vs_ring
 
 suggestion arithmetic
@@ -12,24 +8,24 @@ suggestion arithmetic
 constants a b c d e : ℚ
 
 lemma test3 : (a * (b + c)) * d = a * (b * d) + a * (c * d) :=
-by rewrite_search {explain := tt, trace_summary := tt, view := no visualiser, metric := edit_distance}
+by rewrite_search {explain := tt, trace_summary := tt, no visualiser, metric.edit_distance {}}
 
 lemma test4_ring : (a * (b + c + 1)) * d = a * (b * d) + a * (1 * d) + a * (c * d) :=
 by ring
 
 lemma test4 : (a * (b + c + 1)) * d = a * (b * d) + a * (1 * d) + a * (c * d) :=
-by rewrite_search {explain := tt, trace_summary := tt, view := no visualiser, metric := edit_distance {refresh_freq := 3} weight.cm, strategy := pexplore, max_iterations := 100}
+by rewrite_search {explain := tt, trace_summary := tt, no visualiser, metric.edit_distance {refresh_freq := 3} cm, strategy := pexplore, max_iterations := 100}
 
 lemma test5_ring : (a * (b + c + 1) / e) * d = a * (b / e * d) + a * (1 / e * d) + a * (c / e * d) :=
 by ring
 
 -- lemma test5 : (a * (b + c + 1) / e) * d = a * (b / e * d) + a * (1 / e * d) + a * (c / e * d) :=
--- by rewrite_search {explain := tt, trace_summary := tt, view := no visualiser}
+-- by rewrite_search {explain := tt, trace_summary := tt, no visualiser}
 
 -- lemma test5_2 : (a * (b + c + 1) / e) * d = a * (b / e * d) + a * (1 / e * d) + a * (c / e * d) :=
--- by rewrite_search [add_comm, add_assoc, mul_one, mul_assoc, /-mul_comm,-/ left_distrib, right_distrib] {explain := tt, trace_summary := tt, view := no visualiser, metric := edit_distance {refresh_freq := 10} weight.cm, strategy := pexplore {pop_size := 5}, max_iterations := 500}
+-- by rewrite_search [add_comm, add_assoc, mul_one, mul_assoc, /-mul_comm,-/ left_distrib, right_distrib] {explain := tt, trace_summary := tt, no visualiser, metric.edit_distance {refresh_freq := 10} cm, strategy.pexplore {pop_size := 5}, max_iterations := 500}
 
 -- lemma test5_bfs : (a * (b + c + 1) / e) * d = a * (b / e * d) + a * (1 / e * d) + a * (c / e * d) :=
--- by rewrite_search [add_comm, add_assoc, mul_one, mul_assoc, /-mul_comm,-/ left_distrib, right_distrib] {explain := tt, trace_summary := tt, view := no visualiser, metric := edit_distance {refresh_freq := 3} weight.svm, strategy := bfs, max_iterations := 2000}
+-- by rewrite_search [add_comm, add_assoc, mul_one, mul_assoc, /-mul_comm,-/ left_distrib, right_distrib] {explain := tt, trace_summary := tt, no visualiser, metric.edit_distance {refresh_freq := 3} svm, strategy := bfs, max_iterations := 2000}
 
 end tidy.rewrite_search.vs_ring
